Example.dfy
@@ -7,36 +7,47 @@ module Example {
 
   method Main() {
     // single characters
-    print(Parse(Digit(), "5")); // Some(5)
-    print(Parse(Digit(), "X")); // None
+    print Parse(Digit(), "5"); // Some(5)
+    print "\n";
+    print Parse(Digit(), "X"); // None
+    print "\n";
     var digitOrLetter: Parser<char> := Or(Digit(), Letter());
-    print(Parse(digitOrLetter, "X")); // Some(X)
-    print(Parse(digitOrLetter, "+")); // None
+    print Parse(digitOrLetter, "X"); // Some(X)
+    print "\n";
+    print Parse(digitOrLetter, "+"); // None
+    print "\n";
 
     // identifiers
     var id: Parser<string> := Seq(Letter(),
                                   ZeroOrMore(digitOrLetter),
                                   (s, ss) => [s] + ss);
-    print(Parse(id, "x23")); // Some(x23)
-    print(Parse(id, "a_s")); // Some(a_s)
-    print(Parse(id, "12a")); // None
+    print Parse(id, "x23"); // Some(x23)
+    print "\n";
+    print Parse(id, "a_s"); // Some(a_s)
+    print "\n";
+    print Parse(id, "12a"); // None
+    print "\n";
 
     // s-expressions
-    var atom: Parser<SExpr> :=
-      Map(SkipOptional(OneOrMore(digitOrLetter), Char(' ')),
-          s => Atom(s));
-    var sexpr: Parser<SExpr> := atom;
-    sexpr :=
-      Or(atom,
-         Map(Skip(Then(Char('('), ZeroOrMore(atom)), Char(')')),
-             l => List(l)));
+    var sexpr: Parser<SExpr> := ZComb((sexp: Parser<SExpr>)
+      reads * requires forall s:string :: sexp.run.requires(s)
+      => (
+      var atom: Parser<SExpr> := Map(OneOrMore(digitOrLetter), s => Atom(s));
+      var lst: Parser<SExpr> :=
+        Skip(Then(Char('('),
+                  Map(ZeroOrMore(sexp), l => List(l))),
+            Char(')'));
+      SkipWS(Or(atom, lst))));
 
-    print(Parse(sexpr, "x23"));     // Some(Atom(x23))
-    print("\n");
-    print(Parse(sexpr, "(a b c)")); // Some(List(Atom(a),Atom(b),Atom(c)))
-    print("\n");
-    print(Parse(sexpr, "((a) b)")); // Some(List(List(Atom(a)),Atom(b)))
-    print("\n");
-    print(Parse(sexpr, "(("));      // None
+    print Parse(sexpr, "x23");     // Some(Atom(x23))
+    print "\n";
+    print Parse(sexpr, "(a b c)"); // Some(List(Atom(a),Atom(b),Atom(c)))
+    print "\n";
+    print Parse(sexpr, "((a) b)"); // Some(List(List(Atom(a)),Atom(b)))
+    print "\n";
+    print Parse(sexpr, "((");      // None
+    print "\n";
+
+    print Parse(ZeroOrMore(sexpr), "a b c"); // Some(List(Atom(a),Atom(b),Atom(c)))
   }
 }
